lemma for 3.2 -- we split p -w->_i-1 q into 3 parts

PDS.thy
@@ -60,6 +60,23 @@ inductive transition_of :: "('state, 'label) transition \<Rightarrow> 'state lis
 
 definition path_with_word' where
   "path_with_word' == {(p,w,ss,q) | p w ss q. (ss,w) \<in> path_with_word \<and> p = hd ss \<and> q = last ss}"
+
+inductive_set path_with_word'' where
+  path_with_word_refl''[iff]: "(p,[],[p],p) \<in> path_with_word''"
+| lpath_step: "(p,\<gamma>,q') \<in> transition_relation \<Longrightarrow> (q',w,ss,q) \<in> path_with_word''
+                           \<Longrightarrow> (p, \<gamma>#w, p#ss, q) \<in> path_with_word''"
+
+lemma path_with_word''_induct_non_empty_word: "(x10, x20, x30, x40) \<in> path_with_word'' \<Longrightarrow> x20 \<noteq> [] \<Longrightarrow>
+(\<And>p \<gamma> q'. (p, \<gamma>, q') \<in> transition_relation \<Longrightarrow> P p [\<gamma>] [p, q'] q') \<Longrightarrow>
+(\<And>p \<gamma> q' w ss q. (p, \<gamma>, q') \<in> transition_relation \<Longrightarrow> w \<noteq> [] \<Longrightarrow> (q', w, ss, q) \<in> path_with_word'' \<Longrightarrow> P q' w ss q \<Longrightarrow> P p (\<gamma> # w) (p # ss) q) \<Longrightarrow> P x10 x20 x30 x40"
+proof (induction rule: path_with_word''.induct)
+  case (path_with_word_refl'' p)
+  then show ?case by auto
+next
+  case (lpath_step p \<gamma> q' w ss q)
+  then show ?case
+    by (smt (verit, ccfv_SIG) list.distinct(1) path_with_word''.cases)
+qed
                                                   
 lemma path_with_word_not_empty[simp]: "\<not>([],w) \<in> path_with_word"
   using path_with_word.cases by force
@@ -83,6 +100,19 @@ lemma lpath_path_with_word':
   assumes "(p, w, q) \<in> lpath"
   shows "\<exists>ss. (p, w, ss, q) \<in> path_with_word'"
   using assms lpath_path_with_word unfolding path_with_word'_def by force
+
+lemma lpath_path_with_word'':
+  assumes "(p, w, q) \<in> lpath"
+  shows "\<exists>ss. (p, w, ss, q) \<in> path_with_word''"
+  using assms 
+proof (induction rule: lpath.induct)
+  case (lpath_refl p)
+  then show ?case by auto
+next
+  case (lpath_step p \<gamma> q' w q)
+  then show ?case
+    by (meson LTS.path_with_word''.lpath_step)
+qed
 
 lemma path_with_word_lpath:
   assumes "(ss, w) \<in> path_with_word"
@@ -493,6 +523,20 @@ lemma lemma_3_2_b_aux'': (* Morten's lemma 2*) (* Should this say something abou
   using lemma_3_2_b_aux' 
   sorry
 
+lemma lemma_3_2_b_aux''': (* Morten's lemma 3*) (* Should this say something about ss also? *)
+  assumes "(p, w, ss, q) \<in> LTS.path_with_word'' A"
+  assumes "\<nexists>q \<gamma> q'. (q, \<gamma>, q') \<in> A \<and> q' \<in> P_locs"
+  assumes "q \<in> P_locs"
+  shows "w = [] \<and> p = q"
+  using assms 
+proof(induction rule: LTS.path_with_word''.induct[OF assms(1)])
+  case (1 p)
+  then show ?case by auto
+next
+  case (2 p \<gamma> q' w ss q)
+  then show ?case by auto
+qed
+
 lemma count_next_0:
   assumes "count (transitions_of (s # s' # ss, l # w)) (p1, \<gamma>, q') = 0"
   shows "count (transitions_of (s' # ss, w)) (p1, \<gamma>, q') = 0"
@@ -538,17 +582,184 @@ lemma lemma_3_2_a'_Aux_2:
   apply auto
   done
 
+lemma lemma_3_2_a'_Aux_3:
+  assumes "(p, w, ss ,q) \<in> LTS.path_with_word'' Ai"
+  assumes "0 = count (transitions_of' (p, w, ss, q)) (p1, \<gamma>, q')"
+  assumes "Ai = Aiminus1 \<union> {(p1, \<gamma>, q')}"
+  shows "(p, w, ss, q) \<in> LTS.path_with_word'' Aiminus1"
+  sorry
+
+lemma count_empty_zero: "count (transitions_of' (p, [], [p_add], p_add)) (p1, \<gamma>, q') = 0"
+  by simp
+
+lemma ajskdlfjsla:
+  assumes "(p, \<gamma>', q'_add) \<noteq> (p1, \<gamma>, q')"
+  shows "count (transitions_of' (p, \<gamma>' # w, p # q'_add # ss_rest, q)) (p1, \<gamma>, q') = count (transitions_of' (q'_add, w, q'_add # ss_rest, q)) (p1, \<gamma>, q')"
+  apply (cases w)
+  subgoal
+    using assms
+    apply auto
+    done
+  subgoal 
+    using assms 
+    apply -
+    apply auto
+    done
+  done
+
+
+lemma guuggugugugugugugugugu:
+  assumes "(p, w, ss, q) \<in> LTS.path_with_word'' Ai"
+  assumes "Suc j' = count (transitions_of' (p, w, ss, q)) (p1, \<gamma>, q')"
+  assumes "(p1, \<gamma>, q') \<notin> Aiminus1"
+  assumes "Ai = Aiminus1 \<union> {(p1, \<gamma>, q')}"
+  shows "\<exists>u v u_ss v_ss. ss = u_ss @ v_ss \<and> w = u @ [\<gamma>] @ v \<and> (p, u, u_ss, p1) \<in> LTS.path_with_word'' Aiminus1 \<and> (p1, [\<gamma>], q') \<in> LTS.lpath Ai \<and> (q', v, v_ss, q) \<in> LTS.path_with_word'' Ai"
+  using assms
+proof(induction arbitrary: p rule: LTS.path_with_word''.induct[OF assms(1)])
+  case (1 p_add p)
+  from 1(2) have "False"
+    using count_empty_zero by auto
+  then show ?case
+    by auto
+next
+  case (2 p_add \<gamma>' q'_add w ss q p)
+  then have p_add_p: "p_add = p"
+    by (meson LTS.path_with_word''.cases list.inject)
+  from p_add_p have f2_1: "(p, \<gamma>', q'_add) \<in> Ai"
+    using 2(1) by auto
+  from p_add_p have f2_4: "(p, \<gamma>' # w, p # ss, q) \<in> LTS.path_with_word'' Ai"
+    using 2(4) by auto  
+  from p_add_p have f2_5: "Suc j' = count (transitions_of' (p, \<gamma>' # w, p # ss, q)) (p1, \<gamma>, q')"
+    using 2(5) by auto
+  note f2 = f2_1 2(2) 2(3) f2_4 f2_5 2(6) 2(7)
+  show ?case
+  proof(cases "(p, \<gamma>', q'_add) = (p1, \<gamma>, q')")
+    case True
+    define u :: "'b list" where "u = []"
+    define u_ss :: "'a list" where "u_ss = [p]"
+    define v where "v = w"
+    define v_ss where "v_ss = ss"
+    have "(p, u, u_ss, p1) \<in> LTS.path_with_word'' Aiminus1"
+      using f2 unfolding u_def u_ss_def using LTS.path_with_word''.intros
+      using True by fastforce 
+    have "(p1, [\<gamma>], q') \<in> LTS.lpath Ai"
+      using f2_1
+      by (metis LTS.lpath.lpath_refl LTS.lpath.lpath_step True) 
+    have "(q', v, v_ss, q) \<in> LTS.path_with_word'' Ai"
+      using f2(2)
+      using True v_def v_ss_def by blast
+    show ?thesis
+      by (metis (no_types, lifting) Pair_inject True \<open>(p, u, u_ss, p1) \<in> LTS.path_with_word'' Aiminus1\<close> \<open>(p1, [\<gamma>], q') \<in> LTS.lpath Ai\<close> \<open>(q', v, v_ss, q) \<in> LTS.path_with_word'' Ai\<close> append_Cons p_add_p self_append_conv2 u_def u_ss_def v_def v_ss_def)
+  next
+    case False
+    have "hd ss = q'_add"
+      by (metis LTS.path_with_word''.cases f2(2) list.sel(1))
+    from this False have g: "Suc j' = count (transitions_of' (q'_add, w, ss, q)) (p1, \<gamma>, q')"
+      using f2(5)  
+      apply (cases ss)
+      using ajskdlfjsla
+       apply auto
+      done
+    have "\<exists>u_ih v_ih u_ss_ih v_ss_ih. ss = u_ss_ih @ v_ss_ih \<and> w = u_ih @ [\<gamma>] @ v_ih \<and> (q'_add, u_ih, u_ss_ih, p1) \<in> LTS.path_with_word'' Aiminus1 \<and> (p1, [\<gamma>], q') \<in> LTS.lpath Ai \<and> (q', v_ih, v_ss_ih, q) \<in> LTS.path_with_word'' Ai"
+      using f2(3)[of q'_add, OF f2(2) g f2(6) f2(7)] .
+    then obtain u_ih v_ih u_ss_ih v_ss_ih where ppp:
+      "ss = u_ss_ih @ v_ss_ih" 
+      "w = u_ih @ [\<gamma>] @ v_ih"
+      "(q'_add, u_ih, u_ss_ih, p1) \<in> LTS.path_with_word'' Aiminus1" 
+      "(p1, [\<gamma>], q') \<in> LTS.lpath Ai" 
+      "(q', v_ih, v_ss_ih, q) \<in> LTS.path_with_word'' Ai"
+      by metis
+    define v where "v = v_ih"
+    define v_ss where "v_ss = v_ss_ih"
+    define u where "u = \<gamma>' # u_ih"
+    define u_ss where "u_ss = p # u_ss_ih"
+    have "p_add # ss = u_ss @ v_ss"
+      by (simp add: p_add_p ppp(1) u_ss_def v_ss_def)
+    have "\<gamma>' # w = u @ [\<gamma>] @ v"
+      using ppp(2) u_def v_def by auto
+    have "(p, u, u_ss, p1) \<in> LTS.path_with_word'' Aiminus1"
+      using False LTS.path_with_word''.lpath_step f2(7) f2_1 ppp(3) u_def u_ss_def by fastforce
+    have "(p1, [\<gamma>], q') \<in> LTS.lpath Ai"
+      by (simp add: ppp(4))
+    have "(q', v, v_ss, q) \<in> LTS.path_with_word'' Ai"
+      by (simp add: ppp(5) v_def v_ss_def)
+    show ?thesis
+      apply (rule_tac x=u in exI)
+      apply (rule_tac x=v in exI)
+      apply (rule_tac x=u_ss in exI)
+      apply (rule_tac x=v_ss in exI)
+      using \<open>(p, u, u_ss, p1) \<in> LTS.path_with_word'' Aiminus1\<close> \<open>(q', v, v_ss, q) \<in> LTS.path_with_word'' Ai\<close> \<open>\<gamma>' # w = u @ [\<gamma>] @ v\<close> \<open>p_add # ss = u_ss @ v_ss\<close> ppp(4) by blast
+  qed
+qed
+
+
+(*
+
+
+  case (1 p'' \<gamma>'' q'')
+  then show ?case
+    apply (cases "(p'', \<gamma>'', q'') = (p1, \<gamma>, q')")
+    subgoal
+      apply (rule_tac x="[]" in exI)
+      apply (rule_tac x="[]" in exI)
+      apply (rule_tac x="[p'']" in exI)
+      apply (rule_tac x="[q'']" in exI)
+      apply rule
+      subgoal
+        apply auto 
+        done
+      subgoal
+        apply rule
+        subgoal
+          apply auto
+          done
+        subgoal
+          apply rule
+          subgoal
+            apply (simp add: LTS.path_with_word''.path_with_word_refl'')
+            done
+          subgoal
+            apply rule
+            subgoal
+              apply (metis LTS.lpath.lpath_refl LTS.lpath.lpath_step)
+              done
+            subgoal
+              apply (simp add: LTS.path_with_word''.path_with_word_refl'')
+              done
+            done
+          done
+        done
+      done
+    subgoal
+      apply (subgoal_tac "(p'', \<gamma>'', q'') \<in> Aiminus1")
+      subgoal
+
+        apply (rule_tac x="[]" in exI)
+        apply (rule_tac x="[]" in exI)
+        apply (rule_tac x="[]" in exI)
+        apply (rule_tac x="[]" in exI)
+        sorry
+      subgoal
+        apply blast
+        done
+    done
+  
+next
+  case (2 p \<gamma> q' w ss q)
+  then show ?case sorry
+qed *)
+
 
 lemma lemma_3_2_a':
   assumes "\<nexists>q \<gamma> q'. (q, \<gamma>, q') \<in> A \<and> q' \<in> P_locs"
   assumes "saturation_rule\<^sup>*\<^sup>* A A'"
-  assumes "(p, w, ss, q) \<in> LTS.path_with_word' A'"
-  shows "\<exists>p' w' ss'. (p', w', ss', q) \<in> LTS.path_with_word' A \<and> (p, w) \<Rightarrow>\<^sup>* (p', w')"
+  assumes "(p, w, ss, q) \<in> LTS.path_with_word'' A'"
+  shows "\<exists>p' w' ss'. (p', w', ss', q) \<in> LTS.path_with_word'' A \<and> (p, w) \<Rightarrow>\<^sup>* (p', w')"
   using assms(2) assms(1,3) 
 proof (induction arbitrary: p q w ss rule: rtranclp_induct)
   case base
   then show ?case
-    unfolding LTS.path_with_word'_def by auto
+    by auto
 next
   case (step Aiminus1 Ai)
 
@@ -556,6 +767,7 @@ next
     "Ai = Aiminus1 \<union> {(p1, \<gamma>, q')}" 
     "(p1, \<gamma>) \<hookrightarrow> (p2, w2)"
     "(p2, op_labels w2, q') \<in> LTS.lpath Aiminus1"
+    "(p1, \<gamma>, q') \<notin> Aiminus1"
     by (meson saturation_rule.cases)
 
   note ss_p = step(5)
@@ -566,20 +778,21 @@ next
   from j_def ss_p show ?case
   proof (induction j arbitrary: p q w ss)
     case 0
-    have "(p, w, ss, q) \<in> LTS.path_with_word' Aiminus1"
-      using lemma_3_2_a'_Aux_2
-      by (metis 0 p1_\<gamma>_p2_w2_q'_p(1) t_def) 
+    have "(p, w, ss, q) \<in> LTS.path_with_word'' Aiminus1"
+      using lemma_3_2_a'_Aux_3
+       p1_\<gamma>_p2_w2_q'_p(1) t_def 0 by fastforce
     then show ?case
       using step.IH step.prems(1) by metis
   next
     case (Suc j')
-    then have "\<exists>u v u_ss v_ss. ss = u_ss@v_ss \<and> w = u@[\<gamma>]@v \<and> (p,u,u_ss,p1) \<in> LTS.path_with_word' Aiminus1 \<and> (p1,[\<gamma>],q') \<in> LTS.lpath Ai \<and> (q',v,v_ss,q) \<in> LTS.path_with_word' Ai"
-      sorry
+    have "\<exists>u v u_ss v_ss. ss = u_ss@v_ss \<and> w = u@[\<gamma>]@v \<and> (p,u,u_ss,p1) \<in> LTS.path_with_word'' Aiminus1 \<and> (p1,[\<gamma>],q') \<in> LTS.lpath Ai \<and> (q',v,v_ss,q) \<in> LTS.path_with_word'' Ai"
+      apply (rule guuggugugugugugugugugu[of p w ss q Ai j' p1 \<gamma> q' Aiminus1])
+      using Suc(2,3) t_def  p1_\<gamma>_p2_w2_q'_p(1,4) t_def by auto
     then obtain u v u_ss v_ss where
       "ss = u_ss@v_ss \<and> w = u@[\<gamma>]@v" 
-      "(p,u,u_ss,p1) \<in> LTS.path_with_word' Aiminus1" 
+      "(p,u,u_ss,p1) \<in> LTS.path_with_word'' Aiminus1" 
       "(p1,[\<gamma>],q') \<in> LTS.lpath Ai" 
-      "(q',v,v_ss,q) \<in> LTS.path_with_word' Ai"
+      "(q',v,v_ss,q) \<in> LTS.path_with_word'' Ai"
       by blast
     have II: "p1 \<in> P_locs"
       sorry
